AutoProof: update to Array translation.

eve/Src/Delivery/studio/tools/autoproof/arrays.bpl
@@ -7,120 +7,135 @@ const unique ARRAY#bool#: Type;
 const unique ARRAY#ref#: Type;
 
 // Fields for default attributes
-const unique ARRAY.lower: Field int;
-const unique ARRAY.upper: Field int;
 const unique ARRAY.count: Field int;
 
 // Special attribute for array content
-const unique $area: Field<beta> [int]beta;
+const unique area: Field<beta> [int]beta;
 
-// Function to check if an integer is in the range of valid array indeces
-function ARRAY.$is_index(h: HeapType, a: ref, i: int) returns (bool) {
-	(h[a, ARRAY.lower] <= i && i <= h[a, ARRAY.upper])
+// Basic functions and procedures
+function fun.ARRAY.count(h: HeapType, a: ref) returns (int) {
+	h[a, ARRAY.count]
 }
-
-// Function to obtain the array item at the i-th position
-function ARRAY.$item<beta>(h: HeapType, a: ref, i: int) returns (beta) {
-	h[a, $area][i]
+function fun.ARRAY.is_index(h: HeapType, a: ref, i: int) returns (bool) {
+	(1 <= i && i <= h[a, ARRAY.count])
 }
-// Axiom to provide necessary triggers
-axiom (forall h: HeapType, a: ref, i: int ::
-			{ ARRAY.$item(h, a, i) }
-			{ h[a, $area][i] }
-		ARRAY.$item(h, a, i) == h[a, $area][i]
-	);
-
-// Invariant for array objects
-function ARRAY.$inv(h: HeapType, a: ref) returns (bool) {
-	(a != Void) ==> (
-		(h[a, ARRAY.lower] == 1) && 
-		(h[a, ARRAY.upper] >= 0) && 
-		(h[a, ARRAY.count] >= 0) && 
-		(h[a, ARRAY.count] == h[a, ARRAY.upper] - h[a, ARRAY.lower] + 1)
-	)
+function fun.ARRAY.item<alpha>(h: HeapType, a: ref, i: int) returns (alpha) {
+	h[a, area][i]
 }
+procedure ARRAY.item<alpha>(a: ref, i: int) returns (result: alpha);
+	requires fun.ARRAY.is_index(Heap, a, i); // pre tag:index_in_bounds
+	ensures result == fun.ARRAY.item(Heap, a, i);
 
-function ARRAY#ref#.$inv(h: HeapType, a: ref, ct: Type) returns (bool) {
-	ARRAY.$inv(h, a) &&
-	(forall i: int :: ARRAY.$is_index(h, a, i) ==> (detachable(h, ARRAY.$item(h, a, i), ct)))
-}
+procedure ARRAY.put<alpha>(a: ref, item: alpha, pos: int);
+	requires fun.ARRAY.is_index(Heap, a, pos); // pre tag:index_in_bounds
+	ensures fun.ARRAY.item(Heap, a, pos) == item;
+	ensures Heap[a, area][pos] == item;
+	modifies Heap;
+	ensures (forall<beta> o: ref, f: Field beta :: (o != a || f != area) ==> (Heap[o, f] == old(Heap)[o, f]));
+	ensures (forall i: int :: (fun.ARRAY.is_index(Heap, a, i) && i != pos) ==> fun.ARRAY.item(Heap, a, i) == old(fun.ARRAY.item(Heap, a, i)));
 
-// Invariant for array objects that store integer values
-function ARRAY#int#.$inv(h: HeapType, a: ref) returns (bool) {
-	ARRAY.$inv(h, a) &&
-	(forall i: int :: ARRAY.$is_index(h, a, i) ==> is_integer_32(ARRAY.$item(h, a, i)))
-}
-
-procedure ARRAY#int#.make(
-			c: ref where attached(Heap, c, ARRAY#int#),
+procedure ARRAY.make(
+			c: ref where (c != Void && Heap[c, allocated]),
 			l: int where is_integer_32(l),
 			u: int where is_integer_32(u)
 		);
-	requires l <= u + 1; // pre line:1
-	ensures Heap[c, ARRAY.lower] == l;
-	ensures Heap[c, ARRAY.upper] == u;
-	ensures ARRAY.$inv(Heap, c);
-	ensures (forall i: int :: ARRAY.$is_index(Heap, c, i) ==> ARRAY.$item(Heap, c, i) == 0);
+	requires l == 1; // pre tag:lower_equals_1
+	requires u >= 0; // pre
+	ensures Heap[c, ARRAY.count] == u;
+	ensures ARRAY.inv(Heap, c);
 	modifies Heap;
-	ensures (forall<beta> o: ref, f: Field beta :: (o != c || (f != ARRAY.lower && f != ARRAY.upper && f != ARRAY.count && f != $area)) ==> (Heap[o, f] == old(Heap)[o, f]));
+	ensures (forall<beta> o: ref, f: Field beta :: ((o != c) || (f == allocated)) ==> (Heap[o, f] == old(Heap)[o, f]));
 
-procedure ARRAY#int#.make_filled(
-			c: ref where attached(Heap, c, ARRAY#int#),
-			l: int where is_integer_32(l),
-			u: int where is_integer_32(u),
-			v: int where is_integer_32(v)
-		);
-	requires l <= u + 1;
-	ensures Heap[c, ARRAY.lower] == l;
-	ensures Heap[c, ARRAY.upper] == u;
-	ensures ARRAY.$inv(Heap, c);
-	ensures (forall i: int :: ARRAY.$is_index(Heap, c, i) ==> ARRAY.$item(Heap, c, i) == v);
-	modifies Heap;
-	ensures (forall<beta> o: ref, f: Field beta :: (o != c) ==> (Heap[o, f] == old(Heap)[o, f]));
-
-procedure ARRAY#int#.put(
-			c: ref where attached(Heap, c, ARRAY#int#),
-			item: int where is_integer_32(item),
-			pos: int where is_integer_32(pos)
-		);
-	requires ARRAY.$is_index(Heap, c, pos); // pre line:1
-	ensures ARRAY.$item(Heap, c, pos) == item;
-	ensures ARRAY.$inv(Heap, c);
-	modifies Heap;
-	ensures (forall<beta> o: ref, f: Field beta :: (o != c || f != $area) ==> (Heap[o, f] == old(Heap)[o, f]));
-	ensures (forall i: int :: (ARRAY.$is_index(Heap, c, i) && i != pos) ==> ARRAY.$item(Heap, c, i) == old(ARRAY.$item(Heap, c, i)));
-
-procedure ARRAY#int#.item(
-			c: ref where attached(Heap, c, ARRAY#int#),
-			pos: int where is_integer_32(pos)
-		) returns (result: int);
-	requires ARRAY.$is_index(Heap, c, pos); // pre line:1
-	ensures result == ARRAY.$item(Heap, c, pos);
-
-procedure ARRAY#int#.count(
-			c: ref where attached(Heap, c, ARRAY#int#)
-		) returns (result: int);
-	ensures result == Heap[c, ARRAY.count];
-
-function fun.ARRAY#int#.count(heap: HeapType, c: ref) returns (int) {
-	heap[c, ARRAY.count]
+function fun.ARRAY.has<alpha>(h: HeapType, c: ref, val: alpha) returns (bool) {
+	(exists i: int :: (fun.ARRAY.is_index(h, c, i) && (fun.ARRAY.item(h, c, i) == val)))
 }
 
-procedure ARRAY#int#.has(
-			c: ref where attached(Heap, c, ARRAY#int#),
-			val: int where is_integer_32(val)
-		) returns (result: bool);
-	ensures result == (exists i: int :: (ARRAY.$is_index(Heap, c, i) && (ARRAY.$item(Heap, c, i) == val)));
-
-axiom (forall heap: HeapType, c: ref :: (fun.ARRAY#int#.count(heap, c) == 0) ==> (!(exists i: int :: ARRAY.$is_index(heap, c, i))));
-
-function fun.ARRAY#int#.has(heap: HeapType, c: ref, val: int) returns (bool) {
-	(exists i: int :: (ARRAY.$is_index(heap, c, i) && (ARRAY.$item(heap, c, i) == val)))
+// Array invariants
+function ARRAY.inv(h: HeapType, a: ref) returns (bool) {
+	(a != Void) ==> (h[a, ARRAY.count] >= 0)
+}
+function ARRAY#ref#.inv(h: HeapType, a: ref, ct: Type) returns (bool) {
+	ARRAY.inv(h, a) &&
+	(forall i: int :: fun.ARRAY.is_index(h, a, i) ==> (detachable(h, fun.ARRAY.item(h, a, i), ct)))
+}
+function ARRAY#int#.inv(h: HeapType, a: ref) returns (bool) {
+	ARRAY.inv(h, a) &&
+	(forall i: int :: fun.ARRAY.is_index(h, a, i) ==> is_integer_32(fun.ARRAY.item(h, a, i)))
+}
+function ARRAY#bool#.inv(h: HeapType, a: ref) returns (bool) {
+	ARRAY.inv(h, a)
 }
 
-function fun.ARRAY#int#.has_not(heap: HeapType, c: ref, val: int) returns (bool) {
-	(forall i: int :: (ARRAY.$is_index(heap, c, i) ==> !(ARRAY.$item(heap, c, i) == val)))
-}
+// procedure ARRAY#int#.make(
+			// c: ref where attached(Heap, c, ARRAY#int#),
+			// l: int where is_integer_32(l),
+			// u: int where is_integer_32(u)
+		// );
+	// requires l <= u + 1; // pre line:1
+	// ensures Heap[c, ARRAY.lower] == l;
+	// ensures Heap[c, ARRAY.upper] == u;
+	// ensures ARRAY.$inv(Heap, c);
+	// ensures (forall i: int :: ARRAY.$is_index(Heap, c, i) ==> ARRAY.$item(Heap, c, i) == 0);
+	// modifies Heap;
+	// ensures (forall<beta> o: ref, f: Field beta :: (o != c || (f != ARRAY.lower && f != ARRAY.upper && f != ARRAY.count && f != $area)) ==> (Heap[o, f] == old(Heap)[o, f]));
+
+// procedure ARRAY#int#.make_filled(
+			// c: ref where attached(Heap, c, ARRAY#int#),
+			// l: int where is_integer_32(l),
+			// u: int where is_integer_32(u),
+			// v: int where is_integer_32(v)
+		// );
+	// requires l <= u + 1;
+	// ensures Heap[c, ARRAY.lower] == l;
+	// ensures Heap[c, ARRAY.upper] == u;
+	// ensures ARRAY.$inv(Heap, c);
+	// ensures (forall i: int :: ARRAY.$is_index(Heap, c, i) ==> ARRAY.$item(Heap, c, i) == v);
+	// modifies Heap;
+	// ensures (forall<beta> o: ref, f: Field beta :: (o != c) ==> (Heap[o, f] == old(Heap)[o, f]));
+
+// procedure ARRAY#int#.put(
+			// c: ref where attached(Heap, c, ARRAY#int#),
+			// item: int where is_integer_32(item),
+			// pos: int where is_integer_32(pos)
+		// );
+	// requires ARRAY.$is_index(Heap, c, pos); // pre line:1
+	// ensures ARRAY.$item(Heap, c, pos) == item;
+	// ensures ARRAY.$inv(Heap, c);
+	// modifies Heap;
+	// ensures (forall<beta> o: ref, f: Field beta :: (o != c || f != $area) ==> (Heap[o, f] == old(Heap)[o, f]));
+	// ensures (forall i: int :: (ARRAY.$is_index(Heap, c, i) && i != pos) ==> ARRAY.$item(Heap, c, i) == old(ARRAY.$item(Heap, c, i)));
+
+// procedure ARRAY#int#.item(
+			// c: ref where attached(Heap, c, ARRAY#int#),
+			// pos: int where is_integer_32(pos)
+		// ) returns (result: int);
+	// requires ARRAY.$is_index(Heap, c, pos); // pre line:1
+	// ensures result == ARRAY.$item(Heap, c, pos);
+
+// procedure ARRAY#int#.count(
+			// c: ref where attached(Heap, c, ARRAY#int#)
+		// ) returns (result: int);
+	// ensures result == Heap[c, ARRAY.count];
+
+// function fun.ARRAY#int#.count(heap: HeapType, c: ref) returns (int) {
+	// heap[c, ARRAY.count]
+// }
+
+// procedure ARRAY#int#.has(
+			// c: ref where attached(Heap, c, ARRAY#int#),
+			// val: int where is_integer_32(val)
+		// ) returns (result: bool);
+	// ensures result == (exists i: int :: (ARRAY.$is_index(Heap, c, i) && (ARRAY.$item(Heap, c, i) == val)));
+
+// axiom (forall heap: HeapType, c: ref :: (fun.ARRAY#int#.count(heap, c) == 0) ==> (!(exists i: int :: ARRAY.$is_index(heap, c, i))));
+
+// function fun.ARRAY#int#.has(heap: HeapType, c: ref, val: int) returns (bool) {
+	// (exists i: int :: (ARRAY.$is_index(heap, c, i) && (ARRAY.$item(heap, c, i) == val)))
+// }
+
+// function fun.ARRAY#int#.has_not(heap: HeapType, c: ref, val: int) returns (bool) {
+	// (forall i: int :: (ARRAY.$is_index(heap, c, i) ==> !(ARRAY.$item(heap, c, i) == val)))
+// }
 
 
 // procedure ARRAY#int#.subarray(
@@ -131,7 +146,7 @@ function fun.ARRAY#int#.has_not(heap: HeapType, c: ref, val: int) returns (bool)
 	// requires 1 <= l && l <= fun.ARRAY#int#.count(Heap, c) + 1;
 	// requires 0 <= u && u <= fun.ARRAY#int#.count(Heap, c);
 // //	requires (l <= u) || (l == u + 1);
-	// ensures (forall o: ref :: old(Heap)[o, $allocated] ==> o != result);
+	// ensures (forall o: ref :: old(Heap)[o, allocated] ==> o != result);
 	// ensures attached(Heap, result, ARRAY^INTEGER_32^);
 	// ensures ARRAY.$inv(Heap, result);
 	// ensures Heap[result, ARRAY.lower] == 1;
@@ -143,15 +158,15 @@ function fun.ARRAY#int#.has_not(heap: HeapType, c: ref, val: int) returns (bool)
 	// ensures (forall<beta> o: ref, f: Field beta :: (o != result) ==> (Heap[o, f] == old(Heap)[o, f]));
 
 
-procedure ARRAY#ref#.make(
-			c: ref where attached(Heap, c, ARRAY#ref#),
-			l: int where is_integer_32(l),
-			u: int where is_integer_32(u)
-		);
-	requires l < u;
-	ensures Heap[c, ARRAY.lower] == l;
-	ensures Heap[c, ARRAY.upper] == u;
-	ensures ARRAY.$inv(Heap, c);
-	ensures (forall i: int :: ARRAY.$is_index(Heap, c, i) ==> ARRAY.$item(Heap, c, i) == Void);
-	modifies Heap;
-	ensures (forall<beta> o: ref, f: Field beta :: (o != c) ==> (Heap[o, f] == old(Heap)[o, f]));
+// procedure ARRAY#ref#.make(
+			// c: ref where attached(Heap, c, ARRAY#ref#),
+			// l: int where is_integer_32(l),
+			// u: int where is_integer_32(u)
+		// );
+	// requires l < u;
+	// ensures Heap[c, ARRAY.lower] == l;
+	// ensures Heap[c, ARRAY.upper] == u;
+	// ensures ARRAY.$inv(Heap, c);
+	// ensures (forall i: int :: ARRAY.$is_index(Heap, c, i) ==> ARRAY.$item(Heap, c, i) == Void);
+	// modifies Heap;
+	// ensures (forall<beta> o: ref, f: Field beta :: (o != c) ==> (Heap[o, f] == old(Heap)[o, f]));
