eve/Src/framework/eiffel2boogie/translation/e2b_boogie_generator.e
@@ -42,15 +42,15 @@ feature -- Basic operations
 			l_filename.set_directory (theory_directory)
 			l_filename.set_file_name ("base_theory.bpl")
 			last_generated_verifier_input.add_boogie_file (l_filename)
--- TODO: re-enable?
---			create l_filename.make
---			l_filename.set_directory (theory_directory)
---			l_filename.set_file_name ("arrays.bpl")
---			last_generated_verifier_input.add_boogie_file (l_filename)
---			create l_filename.make
---			l_filename.set_directory (theory_directory)
---			l_filename.set_file_name ("tuples.bpl")
---			last_generated_verifier_input.add_boogie_file (l_filename)
+
+			create l_filename.make
+			l_filename.set_directory (theory_directory)
+			l_filename.set_file_name ("arrays.bpl")
+			last_generated_verifier_input.add_boogie_file (l_filename)
+			create l_filename.make
+			l_filename.set_directory (theory_directory)
+			l_filename.set_file_name ("tuples.bpl")
+			last_generated_verifier_input.add_boogie_file (l_filename)
 
 			create l_printer.make
 			boogie_universe.process (l_printer)
